upgraded rev to reaches

CM2_REV_HALT_dec.v
@@ -14,6 +14,9 @@ Qed.
 Lemma config_eta (x : Config) : x = (state x, (value1 x, value2 x)).
 Proof. by move: x => [? [? ?]]. Qed.
 
+Definition oiter {X : Type} (f : X -> option X) (n : nat) (x : X) :=
+  Nat.iter n (option_bind f) (Some x).
+
 (* an avid instruction may jump to a valid state (except the first) *)
 Inductive avid (l : nat) : Instruction -> Prop :=
   | avidI p b : S p < l -> avid l (dec b (S p)).
@@ -61,11 +64,16 @@ Definition step' (x: Config) : option Config :=
       if value1 x is 0 then Some (1 + (state x), (0, value2 x)) else None
   end.
 
-Definition multi_step' (n: nat) (x: Config) : option Config :=
-  Nat.iter n (option_bind step') (Some x).
+Definition multi_step' : nat -> Config -> option Config := oiter step'.
 
 Notation step := (CM2.step M).
 Notation multi_step := (CM2.multi_step M).
+Notation terminating := (CM2.terminating M).
+Notation non_terminating := (CM2_facts.non_terminating M).
+Notation reaches := (CM2.reaches M).
+Notation reaches_plus := (CM2_facts.reaches_plus M).
+
+Definition reaches' x y := exists k, multi_step' k x = Some y.
 
 (* step includes step' *)
 Lemma step'_incl x y : step' x = Some y -> step x = Some y.
@@ -83,9 +91,8 @@ Proof.
   move=> /(_ y erefl) -> /=. by apply: step'_incl.
 Qed.
 
-Notation terminating := (CM2.terminating M).
-Definition non_terminating x := forall k, multi_step k x <> None.
-
+Corollary reaches'_incl {x y} : reaches' x y -> reaches x y.
+Proof. move=> [k /multi_step'_incl ?]. by exists k. Qed.
 
 Opaque nth_error.
 Arguments nth_error_In {_ _ _ _}.
@@ -125,6 +132,16 @@ Proof.
       congr Some. congr pair. congr pair; lia.
 Qed.
 
+Corollary reaches'E x y : reaches' x y ->
+  exists n m, value1 y = value1 x + n /\ value2 y = value2 x + m /\ 
+    forall a b, (a > 0 -> value1 x > 0) -> (b > 0 -> value2 x > 0) ->
+      reaches' (state x, (a, b)) (state y, (a + n, b + m)).
+Proof.
+  move=> [k] /multi_step'E [n] [m] [?] [?] H.
+  exists n, m. split; [done|split; [done|]].
+  move=> ????. exists k. by apply: H.
+Qed.
+
 Lemma step'_inc_state x y :
   step' x = Some y -> state y = 1 + (state x).
 Proof.
@@ -135,12 +152,15 @@ Proof.
     all: by move=> [/(f_equal state)] /= <-.
 Qed.
 
+(*
 (* for a reversible machine for each configuration one can compute
    the number of steps until the first jump to 0 *)
 Lemma multi_step'I x : 
   { k & { y | multi_step' k x = Some y /\ 
     (if step y is Some z then state z = 0 \/ length M <= state z else True) } }.
 Proof.
+Admitted.
+
   move Hn: (length M - state x) => n. elim: n x Hn.
   { move=> x ?. exists 0, x. split; first done.
     rewrite /step. by have /nth_error_None -> : (length M <= state x) by lia. }
@@ -154,6 +174,35 @@ Proof.
     move: (reversible_not_avid) Hy => /Forall_forall.
     (* ad hoc, possibly externalize *)
     clear -HM. rewrite /step' /step. case Hi: (nth_error M (state x)) => [i|] H; last done.
+    move: Hi => /nth_error_In /H {H}.
+    move: i => []; first done.
+    move=> [] q H.
+    + move: (value2 x) => [|? ? /=]; first done.
+      suff: not (q = S (q - 1) /\ S (q - 1) < length M) by lia.
+      by move=> [+] /avidI => <-.
+    + move: (value1 x) => [|? ? /=]; first done.
+      suff: not (q = S (q - 1) /\ S (q - 1) < length M) by lia.
+      by move=> [+] /avidI => <-.
+Qed.
+*)
+Corollary reaches'I x : 
+  { y | reaches' x y /\ 
+    (if step y is Some z then state z = 0 \/ length M <= state z else True) }.
+Proof.
+  move Hn: (length M - state x) => n. elim: n x Hn.
+  { move=> x ?. exists x. split; first by exists 0.
+    rewrite /step. by have /nth_error_None -> : (length M <= state x) by lia. }
+  move=> n IH x ?. case Hy: (step' x) => [y|].
+  - move: (Hy) => /step'_inc_state ?.
+    have /IH : (length M - state y = n) by lia.
+    move=> [z] [Hyz ?]. exists z. split; last done.
+    move: Hyz => [k Hk]. exists (1+k).
+    by rewrite /multi_step' /oiter iter_plus /= Hy.
+  - exists x. split; first by exists 0.
+    move: (reversible_not_avid) Hy => /Forall_forall.
+    (* ad hoc, possibly externalize *)
+    clear -HM. rewrite /step' /step.
+    case Hi: (nth_error M (state x)) => [i|] H; last done.
     move: Hi => /nth_error_In /H {H}.
     move: i => []; first done.
     move=> [] q H.
@@ -190,57 +239,53 @@ Proof.
       eexists. split; [reflexivity|move=> /=; lia].
 Qed.
 
+
 (* if (1, 1) f->>t-> (0, 1 + m), then (a, b) t->> (0, a * m + b) *)
-Lemma dec_a_0 k x m : multi_step' k (0, (1, 1)) = Some x -> 
+Lemma dec_a_0 x m : reaches' (0, (1, 1)) x -> 
   step x = Some (0, (0, 1 + m)) ->
-  forall a b, exists k', multi_step k' (0, (a, b)) = Some (0, (0, a * m + b)).
+  forall a b, reaches (0, (a, b)) (0, (0, a * m + b)).
 Proof.
   move=> H1x H2x. elim.
   - move=> b. by exists 0.
-  - move=> a IH b. move: H1x => /multi_step'E [n'] [m'] /= [Hax] [Hbx].
+  - move=> a IH b. move: H1x => /reaches'E [n'] [m'] /= [Hax] [Hbx].
     move=> /(_ (S a) b ltac:(lia) ltac:(lia)).
-    move=> /multi_step'_incl Hk.
-    have [k' {}IH] := IH (m + b).
-    exists (k + (1 + k')).
-    move: Hk => /multi_step_plus ->.
+    move=> /reaches'_incl /reaches_trans. apply.
     have ->: m + a * m + b = a * m + (m + b) by lia.
-    rewrite <- IH. apply: multi_step_plus.
-    move: H2x. rewrite /= /step. case: (nth_error M (state x)); last done.
+    apply: (reaches_trans _ (IH (m + b))).
+    exists 1. move: H2x. rewrite /= /step. case: (nth_error M (state x)); last done.
     move=> [].
-    + move=> c [] /= -> ??. congr Some. congr pair. congr pair; lia.
+    + move=> c []. lia.
     + move=> [] q.
       * move: (value2 x) Hbx => [|bx]; first by lia.
         rewrite Hax. move=> ? []. by lia.
       * move: (value1 x) Hax => [|ax]; first by lia.
-        move=> ? [? ? ?] /=. subst. have ->: n' = 0 by lia.
-        congr Some. congr pair. congr pair; lia.
+        move=> ? [? ? ?] /=. congr (Some (_, (_, _))); lia.
 Qed.
 
+
 (* if (1, 1) f->>t-> (1 + n, 0), then (a, b) t->> (b * n + a, 0) *)
-Lemma dec_b_0 k x n : multi_step' k (0, (1, 1)) = Some x -> 
+Lemma dec_b_0 x n : reaches' (0, (1, 1)) x -> 
   step x = Some (0, (1 + n, 0)) ->
-  forall a b, exists k', multi_step k' (0, (a, b)) = Some (0, (b * n + a, 0)).
+  forall a b, reaches (0, (a, b)) (0, (b * n + a, 0)).
 Proof.
   move=> H1x H2x a b. elim: b a.
   - move=> a. by exists 0.
-  - move=> b IH a. move: H1x => /multi_step'E.
-    move=> [n'] [m'] /= [Hax] [Hbx] /(_ a (S b) ltac:(lia) ltac:(lia)).
-    move=> /multi_step'_incl Hk.
-    have [k' {}IH] := IH (n + a). exists (k + (1 + k')).
-    move: Hk => /multi_step_plus ->.
+  - move=> b IH a. move: H1x => /reaches'E [n'] [m'] /= [Hax] [Hbx].
+    move=> /(_ a (S b) ltac:(lia) ltac:(lia)).
+    move=> /reaches'_incl /reaches_trans. apply.
     have ->: n + b * n + a = b * n + (n + a) by lia.
-    rewrite <- IH. apply: multi_step_plus.
-    move: H2x. rewrite /= /step. case: (nth_error M (state x)); last done.
+    apply: (reaches_trans _ (IH (n + a))).
+    exists 1. move: H2x. rewrite /= /step. case: (nth_error M (state x)); last done.
     move=> [].
-    + move=> c [] /= -> ??. congr Some. congr pair. congr pair; lia.
+    + move=> c [] /=. lia.
     + move=> [] q.
       * move: (value2 x) Hbx => [|bx]; first by lia.
-        move=> ? [? ? ?] /=. subst. have ->: m' = 0 by lia.
-        congr Some. congr pair. congr pair; lia.
+        move=> ? [? ? ?] /=. congr (Some (_, (_, _))); lia.
       * move: (value1 x) Hax => [|ax]; first by lia.
         rewrite Hbx. move=> ? []. by lia.
 Qed.
 
+(*
 (* EXPERIMENT WITH step conditions
 Lemma asd2 x y : step x = Some y -> value2 y < value2 x ->
   value1 x = value1 y /\ value2 x = S (value2 y) /\ 
@@ -275,48 +320,44 @@ Proof.
         rewrite Hbx. move=> ? []. by lia.*)
 Qed.
 *)
-
+*)
 (* if (1, 0) f->>t-> (0, 0), then (a, 0) t->> (0, 0) *)
-Lemma dec_a_0' k x : multi_step' k (0, (1, 0)) = Some x -> 
+Lemma dec_a_0' x : reaches' (0, (1, 0)) x -> 
   step x = Some (0, (0, 0)) ->
-  forall a, exists k', multi_step k' (0, (a, 0)) = Some (0, (0, 0)).
+  forall a, reaches (0, (a, 0)) (0, (0, 0)).
 Proof.
   move=> H1x H2x. elim; first by exists 0.
-  move=> a [k' IH]. move: H1x => /multi_step'E.
+  move=> a IH. move: H1x => /reaches'E.
   move=> [n'] [m'] /= [Hax] [Hbx] /(_ (S a) 0 ltac:(lia) ltac:(lia)).
-  move=> /multi_step'_incl Hk.
-  exists (k + (1 + k')).
-  move: Hk => /multi_step_plus ->.
-  rewrite <- IH. apply: multi_step_plus.
+  move=> /reaches'_incl Hk. apply: (reaches_trans Hk).
   move: H2x => /(step_parallel (state x, (S a + n', m'))) /= /(_ ltac:(lia)).
-  move=> [[pz [az bz]]] [->] /= [<-] ?.
-  congr (Some (_, (_, _))); lia.
+  move=> [[pz [az bz]]] /= [/step_reaches] H [?] ?.
+  apply: (reaches_trans H). subst pz.
+  move: IH. congr reaches. congr (_, (_, _)); lia.
 Qed.
 
+
 (* if (0, 1) f->>t-> (0, 0), then (0, b) t->> (0, 0) *)
-Lemma dec_b_0' k x : multi_step' k (0, (0, 1)) = Some x -> 
+Lemma dec_b_0' x : reaches' (0, (0, 1)) x -> 
   step x = Some (0, (0, 0)) ->
-  forall b, exists k', multi_step k' (0, (0, b)) = Some (0, (0, 0)).
+  forall b, reaches (0, (0, b)) (0, (0, 0)).
 Proof.
   move=> H1x H2x. elim; first by exists 0.
-  move=> b [k' IH]. move: H1x => /multi_step'E.
+  move=> b IH. move: H1x => /reaches'E.
   move=> [n'] [m'] /= [Hax] [Hbx] /(_ 0 (S b) ltac:(lia) ltac:(lia)).
-  move=> /multi_step'_incl Hk.
-  exists (k + (1 + k')).
-  move: Hk => /multi_step_plus ->.
-  rewrite <- IH. apply: multi_step_plus.
+  move=> /reaches'_incl Hk. apply: (reaches_trans Hk).
   move: H2x => /(step_parallel (state x, (n', S b + m'))) /= /(_ ltac:(lia)).
-  move=> [[pz [az bz]]] [->] /= [<-] ?.
-  congr (Some (_, (_, _))); lia.
+  move=> [[pz [az bz]]] /= [/step_reaches] H [?] ?.
+  apply: (reaches_trans H). subst pz.
+  move: IH. congr reaches. congr (_, (_, _)); lia.
 Qed.
 
 (* if (1, 1) ->> (S a, S b), then (a', b') does not terminate *)
-Lemma dec_loop k x n m : multi_step' k (0, (1, 1)) = Some x -> 
+Lemma dec_loop x n m : reaches' (0, (1, 1)) x -> 
   step x = Some (0, (1 + n, 1 + m)) ->
   forall a b, non_terminating (0, (a, b)).
 Proof.
-  move=> Hk Hx.
-  move=> a b k' /(multi_step_k_monotone (k' * S k)) /(_ ltac:(lia)).
+  move=> [k Hk] Hx a b k' /(multi_step_k_monotone (k' * S k)) /(_ ltac:(lia)).
   elim: k' a b; first done.
   move=> k' IH a b. have ->: S k' * S k = (k + 1) + (k' * S k) by lia.
   have : multi_step (k + 1) (0, (a, b)) = Some (0, (n + a, b + m)).
@@ -340,18 +381,33 @@ Proof.
     move=> /multi_step_plus ->. by apply: IH.
 Qed.
 
+(*
 (* x f->> HALT (without jumps) *)
 Lemma multi_step'_None_terminating k x y :
   multi_step' k x = Some y -> step y = None ->
   forall a b, (a > 0 -> value1 x > 0) -> (b > 0 -> value2 x > 0) -> 
     terminating (state x, (a, b)).
 Proof.
-  move=> Hx /step_None Hy a b ? ?. exists (1+k).
+  move=> Hx /step_None Hy a b ? ?. exists (k+1).
   move: Hx => /multi_step'E [n] [m] /= [?] [?].
-  move=> /(_ a b ltac:(lia) ltac:(lia)) /multi_step'_incl ->.
-  by apply /step_None.
+  move=> /(_ a b ltac:(lia) ltac:(lia)) /multi_step'_incl.
+  move=> /multi_step_plus ->. by apply /step_None.
+Qed.
+*)
+
+Lemma reaches'_None_terminating x y :
+  reaches' x y -> step y = None ->
+  forall a b, (a > 0 -> value1 x > 0) -> (b > 0 -> value2 x > 0) -> 
+    terminating (state x, (a, b)).
+Proof.
+  move=> Hx /step_None Hy a b ? ?.
+  move: Hx => /reaches'E [n] [m] /= [?] [?].
+  move=> /(_ a b ltac:(lia) ltac:(lia)) /reaches'_incl.
+  move=> /reaches_terminating. apply.
+  exists 1. by apply /step_None.
 Qed.
 
+(*
 (* x f->>t-> HALT (with exactly one jump) *)
 Lemma multi_step'_Some_terminating k x y z :
   multi_step' k x = Some y -> step y = Some z -> length M <= state z ->
@@ -365,9 +421,25 @@ Proof.
   move=> [[pz [az bz]]] [->] /= [<-] ?.
   by apply /step_None /nth_error_None.
 Qed.
+*)
 
-Lemma terminating_orI k p a b x y : 
-  multi_step' k (p, (S a, S b)) = Some x ->
+Lemma reaches'_Some_terminating x y z :
+  reaches' x y -> step y = Some z -> length M <= state z ->
+  forall a b, (value1 x > 0 <-> a > 0) -> (value2 x > 0 <-> b > 0) -> 
+    terminating (state x, (a, b)).
+Proof.
+  move=> Hx Hy Hz a b ? ?.
+  move: Hx => /reaches'E [n] [m] /= [?] [?].
+  move=> /(_ a b ltac:(lia) ltac:(lia)) /reaches'_incl.
+  move: Hy => /(step_parallel (state y, (a + n, b + m))) /= /(_ ltac:(lia)).
+  move=> [[pz [az bz]]] /= [?] [?] ?. subst pz.
+  move=> /reaches_terminating. apply.
+  apply: reaches_terminating; first by (exists 1; eassumption).
+  exists 1. by apply /step_None /nth_error_None.
+Qed.
+
+Lemma terminating_orI p a b x y : 
+  reaches' (p, (S a, S b)) x ->
   step x = Some y ->
   length M <= state y ->
   (forall a', terminating (p, (S a', 0))) + (forall b', terminating (p, (0, S b'))).
@@ -376,51 +448,47 @@ Proof.
   move: i Hi => [].
   { (* inc instruction *)
     move=> c Hx H'x [/(f_equal state) /= H'y] ?. left=> a'.
-    move: H'x => /multi_step'E [n] [m] /= [?] [?].
+    move: H'x => /reaches'E [n] [m] /= [?] [?].
     move=> /(_ (S a') 0 ltac:(lia) ltac:(lia)).
-    move=> /multi_step'_incl Hk.
-    exists (k+2). move: Hk => /multi_step_plus -> /=.
-    rewrite /step /= Hx /=.
+    move=> /reaches'_incl /reaches_terminating. apply.
+    exists 2 => /=. rewrite /step /= Hx /=.
     by have /nth_error_None -> : length M <= S (state x) by lia. }
   (* dec instruction *)
   move=> [] q Hx.
   - move=> +++ /ltac:(right).
-    move=> /multi_step'E [n] [m] /= [->] [->] Hk.
+    move=> /reaches'E [n] [m] /= [->] [->] Hk.
     move=> [/(f_equal state)] /= <- ?.
-    move=> b'. exists (k+2). move: Hk => /(_ 0 (S b') ltac:(lia) ltac:(lia)).
-    move=> /multi_step'_incl /multi_step_plus -> /=.
-    rewrite /step /= Hx /=.
+    move=> b'. move: Hk => /(_ 0 (S b') ltac:(lia) ltac:(lia)).
+    move=> /reaches'_incl /reaches_terminating. apply.
+    exists 2. rewrite /= /step /= Hx /=.
     by have /nth_error_None -> : length M <= q by lia.
   - move=> +++ /ltac:(left).
-    move=> /multi_step'E [n] [m] /= [->] [->] Hk.
+    move=> /reaches'E [n] [m] /= [->] [->] Hk.
     move=> [/(f_equal state)] /= <- ?.
-    move=> a'. exists (k+2). move: Hk => /(_ (S a') 0 ltac:(lia) ltac:(lia)).
-    move=> /multi_step'_incl /multi_step_plus -> /=.
-    rewrite /step /= Hx /=.
+    move=> a'. move: Hk => /(_ (S a') 0 ltac:(lia) ltac:(lia)).
+    move=> /reaches'_incl /reaches_terminating. apply.
+    exists 2. rewrite /= /step /= Hx /=.
     by have /nth_error_None -> : length M <= q by lia.
 Qed.
 
 Lemma transition_loop a b: 
   (forall a' b', (a > 0 <-> a' > 0) -> (b > 0 <-> b' > 0) -> 
-     exists k a'' b'', multi_step k (0, (a', b')) = Some (0, (a'', b'')) /\
-       k > 0 /\ (a' > 0 <-> a'' > 0) /\ (b' > 0 <-> b'' > 0)) ->
+     exists a'' b'', reaches_plus (0, (a', b')) (0, (a'', b'')) /\
+       (a' > 0 <-> a'' > 0) /\ (b' > 0 <-> b'' > 0)) ->
   non_terminating (0, (a, b)).
 Proof.
-  move=> H k. elim: k a b H; first done.
-  move=> k IH a b Hab.
-  have [k' [a' [b' [Hk' ?]]]] := Hab a b ltac:(done) ltac:(done).
-  move=> /(multi_step_k_monotone (k' + k)) /(_  ltac:(lia)).
-  move: Hk' => /multi_step_plus ->. apply: IH.
-  move=> a'' b'' ? ?.
-  have [? [? [? [? ?]]]] := Hab a'' b'' ltac:(lia) ltac:(lia).
-  do 3 eexists. split; first by eassumption.
-  by lia.
+  move=> H. apply: (reaches_plus_invariant_loop 
+    (fun '(p', (a', b')) => p' = 0 /\ (a > 0 <-> a' > 0) /\ (b > 0 <-> b' > 0))); last by lia.
+  move=> [px [ax bx]] [->] H'.
+  move: (H') => [/H] {}H /H [ax'] [bx'] [? ?].
+  exists (0, (ax', bx')). split; [done|lia].
 Qed.
 
+
 (* not (1, 1) f->>t-> (0, 0) *)
-Lemma not_transition_1_1_to_0_0 k x : multi_step' k (0, (1, 1)) = Some x -> step x <> Some (0, (0, 0)).
+Lemma not_transition_1_1_to_0_0 x : reaches' (0, (1, 1)) x -> step x <> Some (0, (0, 0)).
 Proof.
-  move=> /multi_step'E [n] [m] /= [H1x] [H2x] _.
+  move=> /reaches'E [n] [m] /= [H1x] [H2x] _.
   rewrite /step. case: (nth_error M (state x)); last done.
   move=> [].
   - move=> ? [] ?. lia.
@@ -434,39 +502,35 @@ Lemma transition_0_0 :
   (* non-terminating equivalence class (0, 0) *)
   (non_terminating (0, (0, 0))) +
   (* uniform transition to equivalence class (S a, 0) *)
-  (exists k a', multi_step k (0, (0, 0)) = Some (0, (S a', 0))) +
+  (exists a', reaches (0, (0, 0)) (0, (S a', 0))) +
   (* uniform transition to equivalence class (0, S b) *)
-  (exists k b', multi_step k (0, (0, 0)) = Some (0, (0, S b'))) +
+  (exists b', reaches (0, (0, 0)) (0, (0, S b'))) +
   (* uniform transition to equivalence class (S a, S b) *)
-  (exists k a' b', multi_step k (0, (0, 0)) = Some (0, (S a', S b'))).
+  (exists a' b', reaches (0, (0, 0)) (0, (S a', S b'))).
 Proof.
-  have [k [y [Hk]]] := multi_step'I (0, (0, 0)).
+  have [y [/reaches'_incl Hk]] := reaches'I (0, (0, 0)).
   case Hz: (step y) => [[pz [az bz]]|]; first last.
   { (* termination *)
-    move=> _. do 4 left. exists (k+1).
-    by move: Hk => /multi_step'_incl /multi_step_plus ->. }
+    move=> _. do 4 left.
+    move: Hk => /reaches_terminating. apply.
+    by exists 1. }
+  have H0z : reaches_plus (0, (0, 0)) (pz, (az, bz)).
+  { apply: reaches_reaches_plus; [by eassumption|exists 1].
+    split; [lia|done]. }
   case /(eq_or_inf Nat.eq_dec); first last.
   { (* termination *)
-    move=> /nth_error_None H'z. do 4 left. exists (k+(1+1)).
-    move: Hk => /multi_step'_incl /multi_step_plus ->.
-    move: Hz => /(@multi_step_plus M 1) ->.
-    by rewrite /= /step H'z. }
-  move=> /= ?. subst pz.
-  move: az bz Hz => [|az] [|bz] Hz.
+    move=> /nth_error_None H'z. do 4 left.
+    move: H0z => /reaches_plus_incl /reaches_terminating. apply.
+    exists 1. by apply /step_None. }
+  move=> /= ?. subst pz. move: az bz H0z {Hz} => [|az] [|bz] H0z.
   - (* non-termination *)
-    do 3 left. right. move=> a. apply: transition_loop => a' b' ??.
-    exists (k+1), 0, 0.
-    split; last by lia. have ->: a' = 0 by lia. have ->: b' = 0 by lia.
-    by move: Hk => /multi_step'_incl /multi_step_plus ->.
+    do 3 left. right. by apply: reaches_plus_self_loop.
   - (* transition to (0, S b) *)
-    do 1 left. right. exists (k+1), bz.
-    by move: Hk => /multi_step'_incl /multi_step_plus ->.
+    do 1 left. right. exists bz. by apply /reaches_plus_incl.
   - (* transition to (S a, 0) *)
-    do 2 left. right. exists (k+1), az.
-    by move: Hk => /multi_step'_incl /multi_step_plus ->.
+    do 2 left. right. exists az. by apply /reaches_plus_incl.
   - (* transition to (S a, S b) *)
-    right. exists (k+1), az, bz.
-    by move: Hk => /multi_step'_incl /multi_step_plus ->.
+    right. exists az, bz. by apply /reaches_plus_incl.
 Qed.
 
 (* uniform transition from equivalence class (S a, 0) *)
@@ -476,75 +540,68 @@ Lemma transition_Sa_0 :
   (* non-terminating equivalence class (S a, 0) *)
   (forall a, non_terminating (0, (S a, 0))) +
   (* uniform transition to equivalence class (0, 0) *)
-  (forall a, exists k, multi_step k (0, (S a, 0)) = Some (0, (0, 0))) +
+  (forall a, reaches (0, (S a, 0)) (0, (0, 0))) +
   (* uniform transition to equivalence class (0, S b) *)
-  (forall a, exists k b', multi_step k (0, (S a, 0)) = Some (0, (0, S b'))) +
+  (forall a, exists b', reaches (0, (S a, 0)) (0, (0, S b'))) +
   (* uniform transition to equivalence class (S a, S b) *)
-  (forall a, exists k a' b', multi_step k (0, (S a, 0)) = Some (0, (S a', S b'))).
+  (forall a, exists a' b', reaches (0, (S a, 0)) (0, (S a', S b'))).
 Proof.
-  have := multi_step'I (0, (1, 0)).
-  move=> [k'] [x'] [Hx']. case H'x': (step x') => [y'|]; first last.
+  have [x' [Hx']] := reaches'I (0, (1, 0)).
+  case H'x': (step x') => [y'|]; first last.
   { (* case: (1, 0) f->> HALT; uniform termination *)
-    move=> _. do 4 left. move=> a. move: Hx' => /multi_step'_None_terminating.
-    apply => /=; by [assumption|lia]. }
+    move=> _. do 4 left. move=> a. move: Hx' => /reaches'_None_terminating.
+    apply=> /=; by [assumption|lia]. }
   case /(eq_or_inf Nat.eq_dec); first last.
   { (* case: (1, 0) f->>t-> HALT; uniform termination *)
-    move: Hx' H'x' => /multi_step'_Some_terminating H /H {}H /H {}H.
+    move: Hx' H'x' => /reaches'_Some_terminating H /H {}H /H {}H.
     do 4 left. move=> a. apply: H => /=; lia. }
   move: y' H'x' => [py' [ay' [|by']]] + /= Hy'; subst py'.
   { (* case: (1, 0) f->>t-> (_, 0) *)
     move: ay' => [|ay'] H'x'.
     - (* case: (1, 0) f->>t-> (0, 0) uniform transition to (0, 0) *)
-      do 2 left. right. move=> a. apply: dec_a_0'; first by eassumption.
-      by rewrite H'x'.
+      do 2 left. right. move=> a. apply: dec_a_0'; by eassumption.
     - (* non-termination *)
       do 3 left. right. move=> a. apply: transition_loop => a' b' ??.
-      move: Hx' H'x' => /multi_step'E [n] [m] /= [?] [?].
-      move=> /(_ a' b' ltac:(lia) ltac:(lia)) Hk'.
+      move: Hx' H'x' => /reaches'E [n] [m] /= [?] [?].
+      move=> /(_ a' b' ltac:(lia) ltac:(lia)) /reaches'_incl Hk'.
       move=> /(step_parallel (state x', (a' + n, b' + m))) /=.
-      move=> /(_ ltac:(lia)) [[pz [az bz]]] [Hz] /= [? ?].
-      subst pz. exists (k'+1), az, bz.
-      move: Hk' Hz => /multi_step'_incl /multi_step_plus -> /= ->.
-      split; [done|lia]. }
+      move=> /(_ ltac:(lia)) [[pz [az bz]]] [/step_reaches_plus Hz] /= [? ?].
+      subst pz. exists az, bz. split; last by lia.
+      apply: reaches_reaches_plus; by eassumption. }
   move: ay' => [|ay'] H'x'; first last.
   { (* case: (1, 0) f->>t-> (S a, S b) uniform transition to (S a, S b) *)
-    right. move=> a. exists (k'+1).
-    move: Hx' => /multi_step'E [n] [m] /= [Hax'] [Hbx'].
-    move=> /(_ (S a) 0 ltac:(lia) ltac:(lia)) /multi_step'_incl.
+    right. move=> a.
+    move: Hx' => /reaches'E [n] [m] /= [Hax'] [Hbx'].
+    move=> /(_ (S a) 0 ltac:(lia) ltac:(lia)) /reaches'_incl.
     move: H'x' => /(step_parallel (state x', (S a + n, m))) /=.
-    move=> /(_ ltac:(lia)) [[pz' [az' bz']]] /= [Hz'] [? ?].
-    subst pz'. move=> Hx'. exists (az' - 1), (bz' - 1).
-    move: Hx' Hz' => /multi_step_plus -> /= ->.
-    congr Some. congr pair. congr pair; lia. }
+    move=> /(_ ltac:(lia)) [[pz' [az' bz']]] /= [/step_reaches Hz'] [? ?] Hx'.
+    exists (az' - 1), (bz' - 1). apply /(reaches_trans Hx').
+    move: Hz'. congr reaches. congr (_, (_, _)); lia. }
   (* case: (1, 0) f->>t-> (0, S b) *)
-  have := multi_step'I (0, (1, 1)).
-  move=> [k] [x] [Hx]. case H'x: (step x) => [y|]; first last.
+  have := reaches'I (0, (1, 1)).
+  move=> [x] [Hx]. case H'x: (step x) => [y|]; first last.
   { (* case: (1, 1) f->> HALT; uniform termination *)
-    move=> _. do 4 left. move=> a. move: Hx => /multi_step'_None_terminating.
+    move=> _. do 4 left. move=> a. move: Hx => /reaches'_None_terminating.
     apply => /=; by [assumption|lia]. }
   case /(eq_or_inf Nat.eq_dec); first last.
   { (* case: (1, 1) f->>t-> HALT; uniform termination *)
     move=> Hy. move: (Hx) (H'x) (Hy) => /terminating_orI => H /H {}H /H {H} [?|HS]; first by (do 4 left).
     do 4 left. move=> [|a].
-    { move: HS => /(_ by') [k'' ?]. exists (k' + (1 + k'')).
-      move: Hx' => /multi_step'_incl /multi_step_plus ->.
-      by move: H'x' => /(@multi_step_plus M 1) ->. }
-    move: Hx' => /multi_step'E [n] [m] /= [?] [?].
+    { apply: (reaches_terminating _ (HS by')).
+      by apply: (reaches_trans (reaches'_incl Hx') (step_reaches H'x')). }
+    move: Hx' => /reaches'E [n] [m] /= [?] [?].
     move=> /(_ (S (S a)) 0 ltac:(lia) ltac:(lia)).
+    move=> /reaches'_incl /reaches_terminating. apply.
     move: H'x' => /(step_parallel (state x', (S (S a) + n, m))) /=.
-    move=> /(_ ltac:(lia)) [[pz' [az' bz']]] /=.
-    move=> [Hz'] [?] ? Hx'.
-    move: Hx => /multi_step'E [n'] [m'] /= [?] [?].
+    move=> /(_ ltac:(lia)) [[pz' [az' bz']]] /= [Hz'] [?] ?.
+    move: Hz' => /step_reaches /reaches_terminating. apply.
+    subst pz'. move: Hx => /reaches'E [n'] [m'] /= [?] [?].
     move=> /(_ az' bz' ltac:(lia) ltac:(lia)).
+    move=> /reaches'_incl /reaches_terminating. apply.
     move: H'x => /(step_parallel (state x, (az' + n', bz' + m'))) /=.
-    move=> /(_ ltac:(lia)).
-    move=> [z] [Hz] [?] ? Hk. exists (k' + (1 + (k + (1 + 1)))).
-    move: Hx' => /multi_step'_incl /multi_step_plus ->.
-    move: Hz' => /(@multi_step_plus M 1) ->.
-    have ->: pz' = 0 by lia. 
-    move: Hk => /multi_step'_incl /multi_step_plus ->.
-    move: Hz => /(@multi_step_plus M 1) -> /=.
-    apply /step_None /nth_error_None. by lia. }
+    move=> /(_ ltac:(lia)) [z] [Hz] [?] ?.
+    move: Hz => /step_reaches /reaches_terminating. apply.
+    exists 1. apply /step_None /nth_error_None. lia. }
   (* case (1, 1) f->>t-> (a, b) at index 0 *)
   move=> H0y. move Ha'y: (value1 y) => a'y. move Hb'y: (value2 y) => b'y.
   move: a'y b'y Ha'y Hb'y => [|a'y] [|b'y] H1y H2y.
@@ -553,48 +610,40 @@ Proof.
     by rewrite (config_eta y) H0y H1y H2y.
   - (* case: (1, 1) f->>t-> (0, S b') uniform transition to (0, Sb') *)
     do 1 left. right. move=> a.
-    move: Hx' => /multi_step'E [n] [m] /= [?] [?].
-    move=> /(_ (S a) 0 ltac:(lia) ltac:(lia)).
+    move: Hx' => /reaches'E [n] [m] /= [?] [?].
+    move=> /(_ (S a) 0 ltac:(lia) ltac:(lia)) /reaches'_incl Hk'.
     move: H'x' => /(step_parallel (state x', (S a + n, m))) /=.
-    move=> /(_ ltac:(lia)) [y'] [Hy'] [H0y'] ?.
-    move=> /multi_step'_incl Hk'.
+    move=> /(_ ltac:(lia)) [y'] [/step_reaches Hy'] [H0y'] ?.
     move: Hx H'x => /dec_a_0 H. rewrite (config_eta y) H0y H1y H2y.
-    move=> /H {H} => /(_ a (S by')) [k'' Hk''].
-    exists (k' + (1 + k'')), (a * b'y + by').
-    move: Hk' Hy' Hk'' => /multi_step_plus -> /(@multi_step_plus M 1) ->.
-    have ->: y' = (0, (a, S by')).
-    { rewrite (config_eta y') -H0y'. congr pair. congr pair; lia. }
-    move=> ->. congr Some. congr pair. congr pair. lia.
+    move=> /H {H} => /(_ a (S by')) Hk''.
+    exists (a * b'y + by').
+    apply /(reaches_trans Hk') /(reaches_trans Hy').
+    rewrite (config_eta y').
+    move: Hk''. congr reaches; congr (_, (_, _)); lia.
   - (* case: (1, 1) f->>t-> (S a', 0) loop or uniform transition to (0, 0) *)
     move: Hx H'x. rewrite (config_eta y) H0y H1y H2y.
     move=> /dec_b_0 H /H {H}. move: a'y {H1y} => [|a'y] H.
     + (* uniform transition to (0, 0) *)
       do 2 left. right.
-      suff: (forall a, exists k, multi_step k (0, (S a, 0)) = Some (0, (a, 0))).
+      suff: (forall a, reaches (0, (S a, 0)) (0, (a, 0))).
       { clear -HM. move=> H a. elim: (S a); first by exists 0.
-        move=> {}a [k IH]. have [k' Hk'] := H a.
-        exists (k'+k). by move: Hk' => /multi_step_plus ->. }
+        move=> {}a IH. by apply: (reaches_trans (H a) IH). }
       move=> {}a.
-      move: Hx' => /multi_step'E [n] [m] /= [?] [?].
-      move=> /(_ (S a) 0 ltac:(lia) ltac:(lia)) /multi_step'_incl Hk'.
+      move: Hx' => /reaches'E [n] [m] /= [?] [?].
+      move=> /(_ (S a) 0 ltac:(lia) ltac:(lia)) /reaches'_incl.
+      move=> /reaches_trans. apply.
       move: H'x' => /(step_parallel (state x', (S a + n, m))) /=.
       move=> /(_ ltac:(lia)) [[pz [az bz]]] [Hz] /= [? ?].
-      have [k''] := H a (S by'). have ->: S by' * 0 + a = a by lia.
-      move=> Hk''. subst pz. exists (k' + (1 + k'')).
-      move: Hk' => /multi_step_plus ->.
-      move: Hz => /(@multi_step_plus M 1) ->.
-      rewrite -Hk''. congr (multi_step k'' _). congr pair. congr pair; lia.
+      move: Hz => /step_reaches /reaches_trans. apply.
+      move: (H az bz). congr reaches; congr (_, (_, _)); lia.
     + (* non-termination *)
       do 3 left. right. move=> a. apply: transition_loop => a' b' ??.
-      move: Hx' H'x' => /multi_step'E [n] [m] /= [?] [?].
-      move=> /(_ a' b' ltac:(lia) ltac:(lia)) Hk'.
+      move: Hx' H'x' => /reaches'E [n] [m] /= [?] [?].
+      move=> /(_ a' b' ltac:(lia) ltac:(lia)) /reaches'_incl Hk'.
       move=> /(step_parallel (state x', (a' + n, b' + m))) /=.
-      move=> /(_ ltac:(lia)) [[pz [az bz]]] /= [Hz] [? ?]. subst pz.
-      have [k'' Hk''] := H az bz.
-      exists (k'+(1 + k'')), (bz * S a'y + az), 0.
-      move: Hk' Hz Hk'' => /multi_step'_incl /multi_step_plus ->.
-      move=> /(@multi_step_plus M 1) -> ->.
-      split; first done. lia.
+      move=> /(_ ltac:(lia)) [[pz [az bz]]] /= [/step_reaches_plus Hz] [? ?]. subst pz.
+      exists (bz * S a'y + az), 0. split; last by lia.
+      by apply /(reaches_reaches_plus Hk') /(reaches_plus_reaches Hz) /H.
   - (* case: (1, 1) f->>t-> (S a', S b') loop *)
     do 3 left. right. move=> a. apply: dec_loop; [eassumption|].
     by rewrite H'x (config_eta y) H0y H1y H2y.
@@ -607,126 +656,110 @@ Lemma transition_0_Sb :
   (* non-terminating equivalence class*)
   (forall b, non_terminating (0, (0, S b))) +
   (* uniform transition to equivalence class (0, 0) *)
-  (forall b, exists k, multi_step k (0, (0, S b)) = Some (0, (0, 0))) +
+  (forall b, reaches (0, (0, S b)) (0, (0, 0))) +
   (* uniform transition to equivalence class (S a, 0) *)
-  (forall b, exists k a', multi_step k (0, (0, S b)) = Some (0, (S a', 0))) +
+  (forall b, exists a', reaches (0, (0, S b)) (0, (S a', 0))) +
   (* uniform transition to equivalence class (S a, S b) *)
-  (forall b, exists k a' b', multi_step k (0, (0, S b)) = Some (0, (S a', S b'))).
+  (forall b, exists a' b', reaches (0, (0, S b)) (0, (S a', S b'))).
 Proof.
-  have := multi_step'I (0, (0, 1)).
-  move=> [k'] [x'] [Hx']. case H'x': (step x') => [y'|]; first last.
+  have [x' [Hx']] := reaches'I (0, (0, 1)).
+  case H'x': (step x') => [y'|]; first last.
   { (* case: (0, 1) f->> HALT; uniform termination *)
-    move=> _. do 4 left. move=> b. move: Hx' => /multi_step'_None_terminating.
-    apply => /=; by [assumption|lia]. }
+    move=> _. do 4 left. move=> b. move: Hx' => /reaches'_None_terminating.
+    apply=> /=; by [assumption|lia]. }
   case /(eq_or_inf Nat.eq_dec); first last.
   { (* case: (0, 1) f->>t-> HALT; uniform termination *)
-    move: Hx' H'x' => /multi_step'_Some_terminating H /H {}H /H {}H.
+    move: Hx' H'x' => /reaches'_Some_terminating H /H {}H /H {}H.
     do 4 left. move=> b. apply: H => /=; lia. }
   move: y' H'x' => [py' [[|ay'] by']] + /= Hy'; subst py'.
   { (* case: (0, 1) f->>t-> (0, _) *)
     move: by' => [|by'] H'x'.
     - (* case: (0, 1) f->>t-> (0, 0) uniform transition to (0, 0) *)
-      do 2 left. right. move=> b. apply: dec_b_0'; first by eassumption.
-      by rewrite H'x'.
+      do 2 left. right. move=> b. apply: dec_b_0'; by eassumption.
     - (* non-termination *)
       do 3 left. right. move=> b. apply: transition_loop => a' b' ??.
-      move: Hx' H'x' => /multi_step'E [n] [m] /= [?] [?].
-      move=> /(_ a' b' ltac:(lia) ltac:(lia)) Hk'.
+      move: Hx' H'x' => /reaches'E [n] [m] /= [?] [?].
+      move=> /(_ a' b' ltac:(lia) ltac:(lia)) /reaches'_incl Hk'.
       move=> /(step_parallel (state x', (a' + n, b' + m))) /=.
-      move=> /(_ ltac:(lia)) [[pz [az bz]]] [Hz] /= [? ?].
-      subst pz. exists (k'+1), az, bz.
-      move: Hk' Hz => /multi_step'_incl /multi_step_plus -> /= ->.
-      split; [done|lia]. }
+      move=> /(_ ltac:(lia)) [[pz [az bz]]] [/step_reaches_plus Hz] /= [? ?].
+      subst pz. exists az, bz. split; last by lia.
+      apply: reaches_reaches_plus; by eassumption. }
   move: by' => [|by'] H'x'; first last.
   { (* case: (0, 1) f->>t-> (S a, S b) uniform transition to (S a, S b) *)
-    right. move=> b. exists (k'+1).
-    move: Hx' => /multi_step'E [n] [m] /= [Hax'] [Hbx'].
-    move=> /(_ 0 (S b) ltac:(lia) ltac:(lia)) /multi_step'_incl.
+    right. move=> b.
+    move: Hx' => /reaches'E [n] [m] /= [Hax'] [Hbx'].
+    move=> /(_ 0 (S b) ltac:(lia) ltac:(lia)) /reaches'_incl.
     move: H'x' => /(step_parallel (state x', (n, S b + m))) /=.
-    move=> /(_ ltac:(lia)).
-    move=> [[pz' [az' bz']]] /= [Hz'] [? ?]. subst pz'.
-    move=> Hx'. exists (az' - 1), (bz' - 1).
-    move: Hx' Hz' => /multi_step_plus -> /= ->.
-    congr Some. congr pair. congr pair; lia. }
+    move=> /(_ ltac:(lia)) [[pz' [az' bz']]] /= [/step_reaches Hz'] [? ?] Hx'.
+    exists (az' - 1), (bz' - 1). apply /(reaches_trans Hx').
+    move: Hz'. congr reaches. congr (_, (_, _)); lia. }
   (* case: (0, 1) f->>t-> (S a, 0) *)
-  have := multi_step'I (0, (1, 1)).
-  move=> [k] [x] [Hx]. case H'x: (step x) => [y|]; first last.
+  have := reaches'I (0, (1, 1)).
+  move=> [x] [Hx]. case H'x: (step x) => [y|]; first last.
   { (* case: (1, 1) f->> HALT; uniform termination *)
-    move=> _. do 4 left. move=> b. move: Hx => /multi_step'_None_terminating.
+    move=> _. do 4 left. move=> b. move: Hx => /reaches'_None_terminating.
     apply => /=; by [assumption|lia]. }
   case /(eq_or_inf Nat.eq_dec); first last.
   { (* case: (1, 1) f->>t-> HALT; uniform termination *)
     move=> Hy. move: (Hx) (H'x) (Hy) => /terminating_orI => H /H {}H /H {H} [HS|?]; last by (do 4 left).
     do 4 left. move=> [|b].
-    { move: HS => /(_ ay') [k'' ?]. exists (k' + (1 + k'')).
-      move: Hx' => /multi_step'_incl /multi_step_plus ->.
-      by move: H'x' => /(@multi_step_plus M 1) ->. }
-    move: Hx' => /multi_step'E [n] [m] /= [?] [?].
+    { apply: (reaches_terminating _ (HS ay')).
+      by apply: (reaches_trans (reaches'_incl Hx') (step_reaches H'x')). }
+    move: Hx' => /reaches'E [n] [m] /= [?] [?].
     move=> /(_ 0 (S (S b)) ltac:(lia) ltac:(lia)).
+    move=> /reaches'_incl /reaches_terminating. apply.
     move: H'x' => /(step_parallel (state x', (n, S (S b) + m))) /=.
-    move=> /(_ ltac:(lia)) [[pz' [az' bz']]] /=.
-    move=> [Hz'] [?] ? Hx'.
-    move: Hx => /multi_step'E [n'] [m'] /= [?] [?].
+    move=> /(_ ltac:(lia)) [[pz' [az' bz']]] /= [Hz'] [?] ?.
+    move: Hz' => /step_reaches /reaches_terminating. apply.
+    subst pz'. move: Hx => /reaches'E [n'] [m'] /= [?] [?].
     move=> /(_ az' bz' ltac:(lia) ltac:(lia)).
+    move=> /reaches'_incl /reaches_terminating. apply.
     move: H'x => /(step_parallel (state x, (az' + n', bz' + m'))) /=.
-    move=> /(_ ltac:(lia)) [z] [Hz] [?] ? Hk.
-    exists (k' + (1 + (k + (1 + 1)))).
-    move: Hx' => /multi_step'_incl /multi_step_plus ->.
-    move: Hz' => /(@multi_step_plus M 1) ->.
-    have ->: pz' = 0 by lia. 
-    move: Hk => /multi_step'_incl /multi_step_plus ->.
-    move: Hz => /(@multi_step_plus M 1) -> /=.
-    apply /step_None /nth_error_None. by lia. }
+    move=> /(_ ltac:(lia)) [z] [Hz] [?] ?.
+    move: Hz => /step_reaches /reaches_terminating. apply.
+    exists 1. apply /step_None /nth_error_None. lia. }
   (* case (1, 1) f->>t-> (a, b) at index 0 *)
   move=> H0y. move Ha'y: (value1 y) => a'y. move Hb'y: (value2 y) => b'y.
-  move: b'y a'y Hb'y Ha'y => [|b'y] [|a'y] H2y H1y.
+  move: a'y b'y Ha'y Hb'y => [|a'y] [|b'y] H1y H2y.
   - (* case: (1, 1) f->>t-> (0, 0) impossible *)
     move: Hx H'x => /not_transition_1_1_to_0_0.
     by rewrite (config_eta y) H0y H1y H2y.
-  - (* case: (1, 1) f->>t-> (S a', 0) uniform transition to (S a', 0) *)
-    do 1 left. right. move=> b.
-    move: Hx' => /multi_step'E [n] [m] /= [?] [?].
-    move=> /(_ 0 (S b) ltac:(lia) ltac:(lia)).
-    move: H'x' => /(step_parallel (state x', (n, S b + m))) /=.
-    move=> /(_ ltac:(lia)) [y'] [Hy'] [H0y'] ?.
-    move=> /multi_step'_incl Hk'.
-    move: Hx H'x => /dec_b_0 H. rewrite (config_eta y) H0y H1y H2y.
-    move=> /H {H} => /(_ (S ay') b) [k'' Hk''].
-    exists (k' + (1 + k'')), (b * a'y + ay').
-    move: Hk' Hy' Hk'' => /multi_step_plus -> /(@multi_step_plus M 1) ->.
-    have ->: y' = (0, (S ay', b)).
-    { rewrite (config_eta y') -H0y'. congr pair. congr pair; lia. }
-    move=> ->. congr Some. congr pair. congr pair. lia.
   - (* case: (1, 1) f->>t-> (0, S b') loop or uniform transition to (0, 0) *)
     move: Hx H'x. rewrite (config_eta y) H0y H1y H2y.
     move=> /dec_a_0 H /H {H}. move: b'y {H2y} => [|b'y] H.
     + (* uniform transition to (0, 0) *)
       do 2 left. right.
-      suff: (forall b, exists k, multi_step k (0, (0, S b)) = Some (0, (0, b))).
+      suff: (forall b, reaches (0, (0, S b)) (0, (0, b))).
       { clear -HM. move=> H b. elim: (S b); first by exists 0.
-        move=> {}b [k IH]. have [k' Hk'] := H b.
-        exists (k'+k). by move: Hk' => /multi_step_plus ->. }
+        move=> {}b IH. by apply: (reaches_trans (H b) IH). }
       move=> {}b.
-      move: Hx' => /multi_step'E [n] [m] /= [?] [?].
-      move=> /(_ 0 (S b) ltac:(lia) ltac:(lia)) /multi_step'_incl Hk'.
+      move: Hx' => /reaches'E [n] [m] /= [?] [?].
+      move=> /(_ 0 (S b) ltac:(lia) ltac:(lia)) /reaches'_incl.
+      move=> /reaches_trans. apply.
       move: H'x' => /(step_parallel (state x', (n, S b + m))) /=.
       move=> /(_ ltac:(lia)) [[pz [az bz]]] [Hz] /= [? ?].
-      have [k''] := H (S ay') b. have ->: S ay' * 0 + b = b by lia.
-      move=> Hk''. subst pz. exists (k' + (1 + k'')).
-      move: Hk' => /multi_step_plus ->.
-      move: Hz => /(@multi_step_plus M 1) ->.
-      rewrite -Hk''. congr (multi_step k'' _). congr pair. congr pair; lia.
+      move: Hz => /step_reaches /reaches_trans. apply.
+      move: (H az bz). congr reaches; congr (_, (_, _)); lia.
     + (* non-termination *)
       do 3 left. right. move=> b. apply: transition_loop => a' b' ??.
-      move: Hx' H'x' => /multi_step'E [n] [m] /= [?] [?].
-      move=> /(_ a' b' ltac:(lia) ltac:(lia)) Hk'.
+      move: Hx' H'x' => /reaches'E [n] [m] /= [?] [?].
+      move=> /(_ a' b' ltac:(lia) ltac:(lia)) /reaches'_incl Hk'.
       move=> /(step_parallel (state x', (a' + n, b' + m))) /=.
-      move=> /(_ ltac:(lia)) [[pz [az bz]]] /= [Hz] [? ?]. subst pz.
-      have [k'' Hk''] := H az bz.
-      exists (k'+(1 + k'')), 0, (az * S b'y + bz).
-      move: Hk' Hz Hk'' => /multi_step'_incl /multi_step_plus ->.
-      move=> /(@multi_step_plus M 1) -> ->.
-      split; first done. lia.
+      move=> /(_ ltac:(lia)) [[pz [az bz]]] /= [/step_reaches_plus Hz] [? ?]. subst pz.
+      exists 0, (az * S b'y + bz). split; last by lia.
+      by apply /(reaches_reaches_plus Hk') /(reaches_plus_reaches Hz) /H.
+  - (* case: (1, 1) f->>t-> (S a', 0) uniform transition to (S a', 0') *)
+    do 1 left. right. move=> b.
+    move: Hx' => /reaches'E [n] [m] /= [?] [?].
+    move=> /(_ 0 (S b) ltac:(lia) ltac:(lia)) /reaches'_incl Hk'.
+    move: H'x' => /(step_parallel (state x', (n, S b + m))) /=.
+    move=> /(_ ltac:(lia)) [y'] [/step_reaches Hy'] [H0y'] ?.
+    move: Hx H'x => /dec_b_0 H. rewrite (config_eta y) H0y H1y H2y.
+    move=> /H {H} => /(_ (S ay') b) Hk''.
+    exists (b * a'y + ay').
+    apply /(reaches_trans Hk') /(reaches_trans Hy').
+    rewrite (config_eta y').
+    move: Hk''. congr reaches; congr (_, (_, _)); lia.
   - (* case: (1, 1) f->>t-> (S a', S b') loop *)
     do 3 left. right. move=> b. apply: dec_loop; [eassumption|].
     by rewrite H'x (config_eta y) H0y H1y H2y.
@@ -739,37 +772,36 @@ Lemma transition_Sa_Sb :
   (* non-terminating equivalence class (S a, 0) *)
   (forall a b, non_terminating (0, (S a, S b))) +
   (* uniform transition to equivalence class (0, 0) *)
-  (forall a b, exists k, multi_step k (0, (S a, S b)) = Some (0, (0, 0))) +
+  (forall a b, reaches (0, (S a, S b)) (0, (0, 0))) +
   (* uniform transition to equivalence class (S a, 0) *)
-  (forall a b, exists k a', multi_step k (0, (S a, S b)) = Some (0, (S a', 0))) +
+  (forall a b, exists a', reaches (0, (S a, S b)) (0, (S a', 0))) +
   (* uniform transition to equivalence class (0, S b) *)
-  (forall a b, exists k b', multi_step k (0, (S a, S b)) = Some (0, (0, S b'))).
+  (forall a b, exists b', reaches (0, (S a, S b)) (0, (0, S b'))).
 Proof.
-  have := multi_step'I (0, (1, 1)).
-  move=> [k] [x] [Hk]. case H'x: (step x) => [y|]; first last.
+  have := reaches'I (0, (1, 1)).
+  move=> [x] [Hk]. case H'x: (step x) => [y|]; first last.
   { (* case: (1, 1) f->> HALT; uniform termination *)
     move=> _. do 4 left. move=> a b.
-    move: H'x Hk => /multi_step'_None_terminating H /H /=. apply; lia. }
+    move: H'x Hk => /reaches'_None_terminating H /H /=. apply; lia. }
   case /(eq_or_inf Nat.eq_dec); first last.
   { (* case: (1, 0) f->>t-> HALT; uniform termination *)
-    move: H'x Hk => /multi_step'_Some_terminating H /H {}H /H {}H.
+    move: H'x Hk => /reaches'_Some_terminating H /H {}H /H {}H.
     do 4 left. move=> a b. apply: H => /=; lia. }
   move: y H'x => [py' [[|ay'] [|by']]] H'x /= Hy'; subst py'.
   - (* case: (1, 1) f->>t-> (0, 0) impossible *)
     by move: Hk => /not_transition_1_1_to_0_0.
   - (* case: (1, 1) f->>t-> (0, S b) uniform transition to (0, S b) *)
-    right. move=> a b.  
-    move: Hk H'x => /dec_a_0 H /H /(_ (S a) (S b)) [k' Hk'].
-    exists k', (S a * by' + S b - 1).
-    rewrite Hk'. congr Some. congr pair. congr pair; lia.
+    right. move=> a b.
+    move: Hk H'x => /dec_a_0 H /H /(_ (S a) (S b)) Hk'.
+    exists (S a * by' + S b - 1).
+    move: Hk'. congr reaches. congr (_, (_, _)); lia.
   - (* case: (1, 1) f->>t-> (S a, 0) uniform transition to (S a, 0) *)
-    do 1 left. right. move=> a b.  
-    move: Hk H'x => /dec_b_0 H /H /(_ (S a) (S b)) [k' Hk'].
-    exists k', (S b * ay' + S a - 1).
-    rewrite Hk'. congr Some. congr pair. congr pair; lia.
+    do 1 left. right. move=> a b.
+    move: Hk H'x => /dec_b_0 H /H /(_ (S a) (S b)) Hk'.
+    exists (S b * ay' + S a - 1).
+    move: Hk'. congr reaches. congr (_, (_, _)); lia.
   - (* case: (1, 1) f->>t-> (S a, S b) non-termination *)
-    do 3 left. right. move=> a b.
-    apply: dec_loop; by eassumption.
+    do 3 left. right. move=> a b. apply: dec_loop; by eassumption.
 Qed.
 
 (* equivalence class business *)
@@ -788,12 +820,14 @@ Proof.
   - exists (1, 1) => /=. split; [tauto|lia].
 Qed.
 
+(*
 Lemma multi_step_act k x y :
   multi_step k x = Some y -> x <> y -> multi_step (S (k - 1)) x = Some y.
 Proof.
   case: k => [|k] /=; first by congruence.
   by rewrite Nat.sub_0_r.
 Qed.
+*)
 
 Lemma uniform_transition ab :
   In ab representatives -> 
@@ -803,7 +837,7 @@ Lemma uniform_transition ab :
   (forall a'b', RZ ab a'b' -> non_terminating (0, a'b')) +
   (* uniform transition *)
   {v | In v representatives /\
-    (forall a'b', RZ ab a'b' -> exists k w, RZ v w /\ multi_step (S k) (0, a'b') = Some (0, w)) }.
+    (forall a'b', RZ ab a'b' -> exists w, RZ v w /\ reaches_plus (0, a'b') (0, w)) }.
 Proof.
   rewrite /representatives /=.
   have HE := @eq_or_inf (nat * nat) ltac:(by do ? decide equality).
@@ -813,20 +847,17 @@ Proof.
       have ->: a' = 0 by lia. have ->: b' = 0 by lia. done.
     + move=> ?. left. right=> - [a' b'] /= ?. have ->: a' = 0 by lia. have ->: b' = 0 by lia. done.
     + move=> H. right. exists (1, 0). split; first by tauto.
-      move: H => [k] [a'' Hk].      
-      move=> [a' b'] /= ?. have ->: a' = 0 by lia. have ->: b' = 0 by lia.
-      exists (k-1), (S a'', 0). split; first by lia.
-      by move: Hk => /multi_step_act <-.
+      move: H => [a'' Hk] [a' b'] /= ?.
+      have ->: a' = 0 by lia. have ->: b' = 0 by lia.
+      exists (S a'', 0). split; [lia|by apply: (reaches_neq_incl Hk)].
     + move=> H. right. exists (0, 1). split; first by tauto.
-      move: H => [k] [b'' Hk].
-      move=> [a' b'] /= ?. have ->: a' = 0 by lia. have ->: b' = 0 by lia.
-      exists (k-1), (0, S b''). split; first by lia.
-      by move: Hk => /multi_step_act <-.
+      move: H => [b'' Hk] [a' b'] /= ?.
+      have ->: a' = 0 by lia. have ->: b' = 0 by lia.
+      exists (0, S b''). split; [lia|by apply: (reaches_neq_incl Hk)].
     + move=> H. right. exists (1, 1). split; first by tauto.
-      move: H => [k] [a'' [b'' Hk]].
-      move=> [a' b'] /= ?. have ->: a' = 0 by lia. have ->: b' = 0 by lia.
-      exists (k-1), (S a'', S b''). split; first by lia.
-      by move: Hk => /multi_step_act <-.
+      move: H => [a'' [b'' Hk]] [a' b'] /= ?.
+      have ->: a' = 0 by lia. have ->: b' = 0 by lia.
+      exists (S a'', S b''). split; [lia|by apply: (reaches_neq_incl Hk)].
   - have [[[[|]|]|]|] := transition_Sa_0.
     + move=> ?. left. left=> - [a' b'] /= ?.
       have ->: a' = S (a' - 1) by lia. have ->: b' = 0 by lia. done.
@@ -834,18 +865,14 @@ Proof.
       have ->: a' = S (a' - 1) by lia. have ->: b' = 0 by lia. done.
     + move=> H. right. exists (0, 0). split; first by tauto.
       move=> [a' b'] /= ?. have ->: a' = S (a' - 1) by lia. have ->: b' = 0 by lia.
-      have [k Hk] := H (a'-1). exists (k-1), (0, 0). split; first by lia.
-      by move: Hk => /multi_step_act <-.
+      have Hk := H (a'-1). exists (0, 0). split; [lia|by apply: (reaches_neq_incl Hk)].
     + move=> H. right. exists (0, 1). split; first by tauto.
       move=> [a' b'] /= ?. have ->: a' = S (a' - 1) by lia. have ->: b' = 0 by lia.
-      have [k [b'' Hk]] := H (a'-1).
-      exists (k-1), (0, S b''). split; first by lia.
-      by move: Hk => /multi_step_act <-.
+      have [b'' Hk] := H (a'-1). exists (0, S b''). split; [lia|by apply: (reaches_neq_incl Hk)].
     + move=> H. right. exists (1, 1). split; first by tauto.
       move=> [a' b'] /= ?. have ->: a' = S (a' - 1) by lia. have ->: b' = 0 by lia.
-      have [k [a'' [b'' Hk]]] := H (a'-1).
-      exists (k-1), (S a'', S b''). split; first by lia.
-      by move: Hk => /multi_step_act <-.
+      have [a'' [b'' Hk]] := H (a'-1).
+      exists (S a'', S b''). split; [lia|by apply: (reaches_neq_incl Hk)].
   - have [[[[|]|]|]|] := transition_0_Sb.
     + move=> ?. left. left=> - [a' b'] /= ?.
       have ->: a' = 0 by lia. have ->: b' = S (b' - 1) by lia. done.
@@ -853,18 +880,14 @@ Proof.
       have ->: a' = 0 by lia. have ->: b' = S (b' - 1) by lia. done.
     + move=> H. right. exists (0, 0). split; first by tauto.
       move=> [a' b'] /= ?. have ->: a' = 0 by lia. have ->: b' = S (b' - 1) by lia.
-      have [k Hk] := H (b'-1). exists (k-1), (0, 0). split; first by lia.
-      by move: Hk => /multi_step_act <-.
+      have Hk := H (b'-1). exists (0, 0). split; [lia|by apply: (reaches_neq_incl Hk)].
     + move=> H. right. exists (1, 0). split; first by tauto.
       move=> [a' b'] /= ?. have ->: a' = 0 by lia. have ->: b' = S (b' - 1) by lia.
-      have [k [a'' Hk]] := H (b'-1).
-      exists (k-1), (S a'', 0). split; first by lia.
-      by move: Hk => /multi_step_act <-.
+      have [a'' Hk] := H (b'-1). exists (S a'', 0). split; [lia|by apply: (reaches_neq_incl Hk)].
     + move=> H. right. exists (1, 1). split; first by tauto.
       move=> [a' b'] /= ?. have ->: a' = 0 by lia. have ->: b' = S (b' - 1) by lia.
-      have [k [a'' [b'' Hk]]] := H (b'-1).
-      exists (k-1), (S a'', S b''). split; first by lia.
-      by move: Hk => /multi_step_act <-.
+      have [a'' [b'' Hk]] := H (b'-1).
+      exists (S a'', S b''). split; [lia|by apply: (reaches_neq_incl Hk)].
   - have [[[[|]|]|]|] := transition_Sa_Sb.
     + move=> ?. left. left=> - [a' b'] /= ?.
       have ->: a' = S (a' - 1) by lia. have ->: b' = S (b' - 1) by lia. done.
@@ -872,32 +895,28 @@ Proof.
       have ->: a' = S (a' - 1) by lia. have ->: b' = S (b' - 1) by lia. done.
     + move=> H. right. exists (0, 0). split; first by tauto.
       move=> [a' b'] /= ?. have ->: a' = S (a' - 1) by lia. have ->: b' = S (b' - 1) by lia.
-      have [k Hk] := H (a'-1) (b'-1). exists (k-1), (0, 0). split; first by lia.
-      by move: Hk => /multi_step_act <-.
+      have Hk := H (a'-1) (b'-1). exists (0, 0). split; [lia|by apply: (reaches_neq_incl Hk)].
     + move=> H. right. exists (1, 0). split; first by tauto.
       move=> [a' b'] /= ?. have ->: a' = S (a' - 1) by lia. have ->: b' = S (b' - 1) by lia.
-      have [k [a'' Hk]] := H (a'-1) (b'-1).
-      exists (k-1), (S a'', 0). split; first by lia.
-      by move: Hk => /multi_step_act <-.
+      have [a'' Hk] := H (a'-1) (b'-1).
+      exists (S a'', 0). split; [lia|by apply: (reaches_neq_incl Hk)].
     + move=> H. right. exists (0, 1). split; first by tauto.
       move=> [a' b'] /= ?. have ->: a' = S (a' - 1) by lia. have ->: b' = S (b' - 1) by lia.
-      have [k [b'' Hk]] := H (a'-1) (b'-1).
-      exists (k-1), (0, S b''). split; first by lia.
-      by move: Hk => /multi_step_act <-.
+      have [b'' Hk] := H (a'-1) (b'-1).
+      exists (0, S b''). split; [lia|by apply: (reaches_neq_incl Hk)].
 Qed.
 
 Opaque representatives.
-Opaque CM2.multi_step.
-Arguments incl_cons_inv {_ _ _ _}.
+
 
 Lemma RZ_loop v : 
   (forall ab, RZ v ab ->
-    exists k a'b', RZ v a'b' /\ multi_step (S k) (0, ab) = Some (0, a'b')) ->
+    exists a'b', RZ v a'b' /\ reaches_plus (0, ab) (0, a'b')) ->
   forall ab, RZ v ab -> non_terminating (0, ab).
 Proof.
   move=> Hv ab Hab k. elim: k ab Hab; first done.
-  move=> k IH ab /Hv [k'] [a'b'] [/IH] Hk Hk'.
-  move=> /(multi_step_k_monotone (S k' + k)) /(_ ltac:(lia)).
+  move=> k IH ab /Hv [a'b'] [/IH] Hk [k' [? Hk']].
+  move=> /(multi_step_k_monotone (k' + k)) /(_ ltac:(lia)).
   move: Hk' => /multi_step_plus ->. by apply: Hk.
 Qed.
 
@@ -913,37 +932,31 @@ Proof.
     (forall v, In v representatives -> 
     (forall ab, RZ v ab -> terminating (0, ab)) + (forall ab, RZ v ab -> non_terminating (0, ab)) +
     { w | In w L /\
-      (forall ab, RZ v ab -> exists k a'b', RZ w a'b' /\ multi_step (S k) (0, ab) = Some (0, a'b')) } ) }.
+      (forall ab, RZ v ab -> exists a'b', RZ w a'b' /\ reaches_plus (0, ab) (0, a'b')) } ) }.
   { exists representatives; first done. by apply: uniform_transition. }
   case. elim.
   { move=> _ H v /H /= [[|]|]; [tauto|tauto|]. by move=> [?] []. }
-  move=> v0 L IH /incl_cons_inv [Hv0 HL] HRZ. apply: IH; first done.
+  move=> v0 L IH /(@incl_cons_inv (nat*nat)) [Hv0 HL] HRZ. apply: IH; first done.
   move=> v /HRZ. move=> [[|]|]; [tauto|tauto|].
   have HE := @eq_or_inf (nat * nat) ltac:(by do ? decide equality).
   move=> [w] /= [/HE [|]]; first last.
   { move=> ??. right. by exists w. }
   move=> <-. move: Hv0 => /HRZ [[|]|].
   - (* termination *)
-    move=> Hv0 Hv. left. left=> ab /Hv [k] [a'b'] [/Hv0].
-    move=> [k' Hk'] HSk. exists ((S k) + k').
-    by move: HSk => /multi_step_plus ->.
+    move=> Hv0 Hv. left. left=> ab /Hv [a'b'] [/Hv0].
+    by move=> /reaches_terminating H /reaches_plus_incl /H.
   - (* non-termination *)
-    move=> Hv0 Hv. left. right=> ab /Hv [k] [a'b'] [/Hv0].
-    move=> Ha'b' HSk k'.
-    move=> /(multi_step_k_monotone ((S k)+k')) /(_ ltac:(lia)).
-    move: HSk => /multi_step_plus ->. by apply: Ha'b'.
+    move=> Hv0 Hv. left. right=> ab /Hv [a'b'] [/Hv0].
+    by move=> /reaches_non_terminating H /reaches_plus_incl /H.
   - (* chaining *)
     move=> [w'] /= [/HE [|]].
     + (* non-termination *)
-      move=> <- /RZ_loop Hv0 Hv. left. right=> ab /Hv [k] [a'b'] [/Hv0].
-      move=> Ha'b' HSk k'.
-      move=> /(multi_step_k_monotone ((S k)+k')) /(_ ltac:(lia)).
-      move: HSk => /multi_step_plus ->. by apply: Ha'b'.
+      move=> <- /RZ_loop Hv0 Hv. left. right=> ab /Hv [a'b'] [/Hv0].
+      by move=> /reaches_non_terminating H /reaches_plus_incl /H.
     + move=> ? Hv0 Hv. right. exists w'. split; first done.
-      move=> ab /Hv [k] [a'b'] [/Hv0] [k'] [a''b''] [? HSk'] HSk.
-      exists (k + (S k')), a''b''. split; first done.
-      have ->: S (k + S k') = (S k) + (S k') by done.
-      by move: HSk => / multi_step_plus ->.
+      move=> ab /Hv [a'b'] [/Hv0] [a''b''] [? HSk'] HSk.
+      exists a''b''. split; first done.
+      by apply: (reaches_plus_trans HSk HSk').
 Qed.
 
 Lemma uniform_decision_0 a b : (terminating (0, (a, b))) + (non_terminating (0, (a, b))).
@@ -954,30 +967,23 @@ Qed.
 
 Lemma uniform_decision (c: Config) : (terminating c) + (non_terminating c).
 Proof.
-  have := multi_step'I c.
-  move=> [k] [y] [Hk].
+  have [y [/reaches'_incl Hk]] := reaches'I c.
   case Hz: (step y) => [[pz [az bz]]|] /=; first last.
   { (* termination *)
-    move=> _. left. exists (k+1).
-    by move: Hk => /multi_step'_incl /multi_step_plus ->. }
+    move=> _. left. apply: (reaches_terminating Hk).
+    by exists 1. }
+  have Hcz : reaches c (pz, (az, bz)).
+  { apply: reaches_trans; [|exists 1]; by eassumption. }
   case /(eq_or_inf Nat.eq_dec); first last.
   { (* termination *)
-    move=> /nth_error_None Hpz. left. exists (k+(1+1)).
-    move: Hk => /multi_step'_incl /multi_step_plus ->.
-    move: Hz => /(@multi_step_plus M 1) ->.
-    by apply /step_None. }
-  move=> ?. subst pz.
-  case: (uniform_decision_0 az bz).
+    move=> /nth_error_None Hpz. left.
+    move: Hcz => /reaches_terminating. apply.
+    exists 1. by apply /step_None. }
+  move=> ?. subst pz. case: (uniform_decision_0 az bz).
   - (* termination *)
-    move=> + /ltac:(left). move=> [k' Hk']. exists (k+(1+k')).
-    move: Hk => /multi_step'_incl /multi_step_plus ->.
-    by move: Hz => /(@multi_step_plus M 1) ->.
+    move=> /reaches_terminating H'z. left. by apply: H'z.
   - (* non-termination *)
-    move=> H'z. right=> k'.
-    move=> /(multi_step_k_monotone (k+(1+k'))) /(_ ltac:(lia)).
-    move: Hk => /multi_step'_incl /multi_step_plus ->.
-    move: Hz => /(@multi_step_plus M 1) ->.
-    by apply: H'z.
+    move=> /reaches_non_terminating H'z. right. by apply: H'z.
 Qed.
 
 End Construction.
